---
mathLink: $(f\circ g)\circ h=f\circ (g\circ h)$  
tags:  
- "Type/Proposition"  
- "Topic/Linear_Algebra"  
- "Class/MATH_31AH"  
---
Proved by: <i>Not Applicable</i>  
References: <i>Not Applicable</i>  
Justifications: <i>Not Applicable</i>  
  
Specializations: <i>Not Applicable</i>  
Generalizations: <i>Not Applicable</i>  
  
> [!proposition] Composition is Associative  
> Composition is associative:  
> $$(f\circ g)\circ h=f\circ (g\circ h)$$  
  
**Proof.**  
$$((f\circ g)\circ h)(x)=(f\circ g)(h(x))=f(g(h(x))),\text{whereas}$$  
$$(f\circ(g\circ h))(x)=f((g\circ h)(x))=f(g(h(x))).$$  
