---  
mathLink: $(AB)^{-1}=B^{-1}A^{-1}$  
tags:  
- "Type/Proposition"  
- "Topic/Linear_Algebra"  
- "Class/MATH_31AH"  
---  
Proved by: <i>Not Applicable</i>  
References: <i>Not Applicable</i>  
Justifications: <i>Not Applicable</i>  
  
Specializations: <i>Not Applicable</i>  
Generalizations: <i>Not Applicable</i>  
  
> [!proposition] Inverse of Product of Matrices  
> If $A$ and $B$ are [[Invertible Matrix|invertible matrices]], then $AB$ is invertible, and the inverse is given by  
> $$(AB)^{-1}=B^{-1}A^{-1}.$$  
  
**Proof.** The computations  
$$(AB)(B^{-1}A^{-1})=A(BB^{-1})A^{-1}=AA^{-1}=I$$  
and  
$$(B^{-1}A^{-1})(AB)=B^{-1}(A^{-1}A)B=B^{-1}B=I$$  
prove the result.  
