---
tags:
- Type/Note
- Topic/Differential_Equations
- Class/MATH_20D
date:
- 2024-01-29
---

> [!note] $g(t)=k\cos(\omega t)\text{ or }g(t)=k\sin(\omega t)\text{ or both}$
> $Y_{P}=A\cos(\omega t)+B\sin(\omega t)$  

> [!note] $g(t)=P_{n}(t)=a_{n}t^n+a_{n-1}t^{n-1}+\dots+a_{1}(t)+a_{0}$
> $Y_{P}=A_{n}t^n+A_{n-1}t^{n-1}+\dots+A_{1}t+A_{0}$  

> [!note] Principle of Superposition
> Let $a\neq 0$ and $g_{1}(t),g_{2}(t)$ be functions. If $Y_{1}$ is a solution to the equation  
> $$ay''+by'+cy=g_{1}(t)$$  
> and $Y_{2}$ is a solution to the equation  
> $$ay''+by'+cy=g_{2}(t)$$  
> then $Y_{1}+Y_{2}$ is a solution to the equation  
> $$ay''+by'+cy=g_{1}(t)+g_{2}(t)$$  

> [!note] $g(t)=P_{n}(t)e^{rt}$
> $Y_{P}=(A_{n}t^n+A_{n-1}t^{n-1}+\dots+A_{1}t+A_{0})e^{rt}$  
> Check for conflict with general solution  

> [!note] $g(t)=P_{n}(t)e^{rt}\cos(\omega t)\text{ or }g(t)=P_{n}(t)e^{rt}\sin(\omega t)$
> $Y_{P}=(A_{n}t^n+A_{n-1}t^{n-1}+\dots+A_{1}t+A_{0})e^{rt}\cos(\omega t)+(B_{n}t^n+B_{n-1}t^{n-1}+\dots+B_{1}t+B_{0})e^{rt}\sin(\omega t)$  
